Fp/Multiplication.lean
@@ -5,7 +5,7 @@ import Fp.Negation
 /--
 Multiplication of two fixed-point numbers.
 -/
-@[bv_float_normalize]
+@[bv_normalize]
 def f_mul (a : FixedPoint v e) (b : FixedPoint w f) : FixedPoint (v+w) (e+f) :=
   let hExOffset := Nat.add_lt_add a.hExOffset b.hExOffset
   let a' : BitVec (v+w) := a.val.setWidth' (by omega)
@@ -19,7 +19,7 @@ def f_mul (a : FixedPoint v e) (b : FixedPoint w f) : FixedPoint (v+w) (e+f) :=
 /--
 Multiplication of two extended fixed-point numbers.
 -/
-@[bv_float_normalize]
+@[bv_normalize]
 def e_mul (a : EFixedPoint v e) (b : EFixedPoint w f) : EFixedPoint (v+w) (e+f) :=
   let hExOffset := Nat.add_lt_add a.num.hExOffset b.num.hExOffset
   open EFixedPoint in
@@ -42,7 +42,7 @@ number using the provided rounding mode.
 
 Implemented using `e_mul`, by conversion to extended fixed-point numbers.
 -/
-@[bv_float_normalize]
+@[bv_normalize]
 def mulfixed
   (a b : PackedFloat e s) (m : RoundingMode) : PackedFloat e s :=
   round _ _ m (e_mul a.toEFixed b.toEFixed)
@@ -53,7 +53,7 @@ number using the provided rounding mode.
 
 A bit-blastable version of multiplication, without using `e_mul`.
 -/
-@[bv_float_normalize]
+@[bv_normalize]
 def mul
   (a b : PackedFloat e s) (m : RoundingMode) : PackedFloat e s :=
   if a.isNaN || b.isNaN ||
@@ -84,7 +84,7 @@ def mul
 /--
 Doubles the given floating point number, rounding to infinity if applicable.
 -/
-@[bv_float_normalize]
+@[bv_normalize]
 def doubleRNE (a : PackedFloat e s) : PackedFloat e s :=
   if a.isNaN then PackedFloat.getNaN _ _
   else if a.isZeroOrSubnorm then
